generate full verif files

examples/cms/verif_Win2.v
@@ -5,6 +5,11 @@ Require Import ProD3.core.Tofino.
 Require Import ProD3.examples.cms.ConModel.
 Require Import ProD3.examples.cms.common.
 Require Import ProD3.examples.cms.ModelRepr.
+Require Import ProD3.examples.cms.verif_Row21.
+Require Import ProD3.examples.cms.verif_Row22.
+Require Import ProD3.examples.cms.verif_Row23.
+Require Import ProD3.examples.cms.verif_Row24.
+Require Import ProD3.examples.cms.verif_Row25.
 Require Import Hammer.Plugin.Hammer.
 Require Export Coq.Program.Program.
 Import ListNotations.
@@ -15,6 +20,680 @@ Notation Val := (@ValueBase bool).
 Notation Sval := (@ValueBase (option bool)).
 
 Definition p := ["pipe"; "ingress"; "cm2_ds"; "win_2"].
+
+Definition P4min a b := Z.min (P4Arith.BitArith.mod_bound value_w a) (P4Arith.BitArith.mod_bound value_w b).
+
+Definition min_spec : func_spec :=
+  WITH,
+    PATH []
+    MOD None []
+    WITH (a b : Z),
+      PRE
+        (ARG [P4Bit value_w a; P4Bit value_w b]
+        (MEM []
+        (EXT [])))
+      POST
+        (ARG_RET [] (P4Bit value_w (P4min a b))
+        (MEM []
+        (EXT []))).
+
+Lemma min_body :
+  func_sound ge (FExternal "" "min") [TypBit value_w] min_spec.
+Admitted.
+
+#[local] Hint Extern 5 (func_modifies _ _ _ _ _) => (apply min_body) : func_specs.
+
+Definition act_merge_rows_1_fd :=
+  ltac:(get_fd ["Cm2CountMinSketchWin"; "act_merge_rows_1"] ge).
+
+Definition act_merge_rows_1_spec : func_spec :=
+  WITH (* p *),
+    PATH p
+    MOD (Some [["win_md"]]) []
+    WITH api index_1 index_2 index_3 index_4 index_5 rw_1 rw_2 rw_3 rw_4 rw_5,
+      PRE
+        (ARG []
+        (MEM [(["win_md"], ValBaseStruct
+               [("api", api);
+                ("index_1", index_1);
+                ("index_2", index_2);
+                ("index_3", index_3);
+                ("index_4", index_4);
+                ("index_5", index_5);
+                ("rw_1", P4Bit value_w rw_1);
+                ("rw_2", P4Bit value_w rw_2);
+                ("rw_3", P4Bit value_w rw_3);
+                ("rw_4", P4Bit value_w rw_4);
+                ("rw_5", P4Bit value_w rw_5)
+               ])
+             ]
+        (EXT [])))
+      POST
+        (ARG_RET [] ValBaseNull
+        (MEM [(["win_md"], ValBaseStruct
+               [("api", api);
+                ("index_1", index_1);
+                ("index_2", index_2);
+                ("index_3", index_3);
+                ("index_4", index_4);
+                ("index_5", index_5);
+                ("rw_1", P4Bit value_w (P4min rw_1 rw_4));
+                ("rw_2", P4Bit value_w (P4min rw_2 rw_5));
+                ("rw_3", P4Bit value_w rw_3);
+                ("rw_4", P4Bit value_w rw_4);
+                ("rw_5", P4Bit value_w rw_5)
+               ])
+             ]
+        (EXT []))).
+
+Lemma act_merge_rows_1_body :
+  func_sound ge act_merge_rows_1_fd nil act_merge_rows_1_spec.
+Proof.
+  start_function.
+  step_call min_body.
+  { entailer. }
+  step_call min_body.
+  { entailer. }
+  step.
+  entailer.
+Qed.
+
+#[local] Hint Extern 5 (func_modifies _ _ _ _ _) => (apply act_merge_rows_1_body) : func_specs.
+
+Definition act_merge_rows_2_fd :=
+  ltac:(get_fd ["Cm2CountMinSketchWin"; "act_merge_rows_2"] ge).
+
+Definition act_merge_rows_2_spec : func_spec :=
+  WITH (* p *),
+    PATH p
+    MOD (Some [["win_md"]]) []
+    WITH api index_1 index_2 index_3 index_4 index_5 rw_1 rw_2 rw_3 rw_4 rw_5,
+      PRE
+        (ARG []
+        (MEM [(["win_md"], ValBaseStruct
+               [("api", api);
+                ("index_1", index_1);
+                ("index_2", index_2);
+                ("index_3", index_3);
+                ("index_4", index_4);
+                ("index_5", index_5);
+                ("rw_1", P4Bit value_w rw_1);
+                ("rw_2", P4Bit value_w rw_2);
+                ("rw_3", P4Bit value_w rw_3);
+                ("rw_4", rw_4);
+                ("rw_5", rw_5)
+               ])
+             ]
+        (EXT [])))
+      POST
+        (ARG_RET [] ValBaseNull
+        (MEM [(["win_md"], ValBaseStruct
+               [("api", api);
+                ("index_1", index_1);
+                ("index_2", index_2);
+                ("index_3", index_3);
+                ("index_4", index_4);
+                ("index_5", index_5);
+                ("rw_1", P4Bit value_w (P4min rw_1 rw_3));
+                ("rw_2", P4Bit value_w rw_2);
+                ("rw_3", P4Bit value_w rw_3);
+                ("rw_4", rw_4);
+                ("rw_5", rw_5)
+               ])
+             ]
+        (EXT []))).
+
+Lemma act_merge_rows_2_body :
+  func_sound ge act_merge_rows_2_fd nil act_merge_rows_2_spec.
+Proof.
+  start_function.
+  step_call min_body.
+  { entailer. }
+  step.
+  entailer.
+Qed.
+
+#[local] Hint Extern 5 (func_modifies _ _ _ _ _) => (apply act_merge_rows_2_body) : func_specs.
+
+Definition act_merge_rows_3_fd :=
+  ltac:(get_fd ["Cm2CountMinSketchWin"; "act_merge_rows_3"] ge).
+
+Definition act_merge_rows_3_spec : func_spec :=
+  WITH (* p *),
+    PATH p
+    MOD (Some [["win_md"]]) []
+    WITH api index_1 index_2 index_3 index_4 index_5 rw_1 rw_2 rw_3 rw_4 rw_5,
+      PRE
+        (ARG []
+        (MEM [(["win_md"], ValBaseStruct
+               [("api", api);
+                ("index_1", index_1);
+                ("index_2", index_2);
+                ("index_3", index_3);
+                ("index_4", index_4);
+                ("index_5", index_5);
+                ("rw_1", P4Bit value_w rw_1);
+                ("rw_2", P4Bit value_w rw_2);
+                ("rw_3", rw_3);
+                ("rw_4", rw_4);
+                ("rw_5", rw_5)
+               ])
+             ]
+        (EXT [])))
+      POST
+        (ARG_RET [] ValBaseNull
+        (MEM [(["win_md"], ValBaseStruct
+               [("api", api);
+                ("index_1", index_1);
+                ("index_2", index_2);
+                ("index_3", index_3);
+                ("index_4", index_4);
+                ("index_5", index_5);
+                ("rw_1", P4Bit value_w (P4min rw_1 rw_2));
+                ("rw_2", P4Bit value_w rw_2);
+                ("rw_3", rw_3);
+                ("rw_4", rw_4);
+                ("rw_5", rw_5)
+               ])
+             ]
+        (EXT []))).
+
+Lemma act_merge_rows_3_body :
+  func_sound ge act_merge_rows_3_fd nil act_merge_rows_3_spec.
+Proof.
+  start_function.
+  step_call min_body.
+  { entailer. }
+  step.
+  entailer.
+Qed.
+
+#[local] Hint Extern 5 (func_modifies _ _ _ _ _) => (apply act_merge_rows_3_body) : func_specs.
+
+Definition tbl_merge_rows_1_fd :=
+  ltac:(get_fd ["Cm2CountMinSketchWin"; "tbl_merge_rows_1"; "apply"] ge).
+
+Definition tbl_merge_rows_1_spec : func_spec :=
+  WITH (* p *),
+    PATH p
+    MOD (Some [["win_md"]]) []
+    WITH api index_1 index_2 index_3 index_4 index_5 rw_1 rw_2 rw_3 rw_4 rw_5,
+      PRE
+        (ARG []
+        (MEM [(["win_md"], ValBaseStruct
+               [("api", api);
+                ("index_1", index_1);
+                ("index_2", index_2);
+                ("index_3", index_3);
+                ("index_4", index_4);
+                ("index_5", index_5);
+                ("rw_1", P4Bit value_w rw_1);
+                ("rw_2", P4Bit value_w rw_2);
+                ("rw_3", P4Bit value_w rw_3);
+                ("rw_4", P4Bit value_w rw_4);
+                ("rw_5", P4Bit value_w rw_5)
+               ])
+             ]
+        (EXT [])))
+      POST
+        (EX retv,
+        (ARG_RET [] retv
+        (MEM [(["win_md"], ValBaseStruct
+               [("api", api);
+                ("index_1", index_1);
+                ("index_2", index_2);
+                ("index_3", index_3);
+                ("index_4", index_4);
+                ("index_5", index_5);
+                ("rw_1", P4Bit value_w (P4min rw_1 rw_4));
+                ("rw_2", P4Bit value_w (P4min rw_2 rw_5));
+                ("rw_3", P4Bit value_w rw_3);
+                ("rw_4", P4Bit value_w rw_4);
+                ("rw_5", P4Bit value_w rw_5)
+               ])
+             ]
+        (EXT []))))%arg_ret_assr.
+
+Lemma tbl_merge_rows_1_body :
+  func_sound ge tbl_merge_rows_1_fd nil tbl_merge_rows_1_spec.
+Proof.
+  start_function.
+  table_action act_merge_rows_1_body.
+  { entailer. }
+  { entailer. }
+Qed.
+
+#[local] Hint Extern 5 (func_modifies _ _ _ _ _) => (apply tbl_merge_rows_1_body) : func_specs.
+
+Definition tbl_merge_rows_2_fd :=
+  ltac:(get_fd ["Cm2CountMinSketchWin"; "tbl_merge_rows_2"; "apply"] ge).
+
+Definition tbl_merge_rows_2_spec : func_spec :=
+  WITH (* p *),
+    PATH p
+    MOD (Some [["win_md"]]) []
+    WITH api index_1 index_2 index_3 index_4 index_5 rw_1 rw_2 rw_3 rw_4 rw_5,
+      PRE
+        (ARG []
+        (MEM [(["win_md"], ValBaseStruct
+               [("api", api);
+                ("index_1", index_1);
+                ("index_2", index_2);
+                ("index_3", index_3);
+                ("index_4", index_4);
+                ("index_5", index_5);
+                ("rw_1", P4Bit value_w rw_1);
+                ("rw_2", P4Bit value_w rw_2);
+                ("rw_3", P4Bit value_w rw_3);
+                ("rw_4", rw_4);
+                ("rw_5", rw_5)
+               ])
+             ]
+        (EXT [])))
+      POST
+        (EX retv,
+        (ARG_RET [] retv
+        (MEM [(["win_md"], ValBaseStruct
+               [("api", api);
+                ("index_1", index_1);
+                ("index_2", index_2);
+                ("index_3", index_3);
+                ("index_4", index_4);
+                ("index_5", index_5);
+                ("rw_1", P4Bit value_w (P4min rw_1 rw_3));
+                ("rw_2", P4Bit value_w rw_2);
+                ("rw_3", P4Bit value_w rw_3);
+                ("rw_4", rw_4);
+                ("rw_5", rw_5)
+               ])
+             ]
+        (EXT []))))%arg_ret_assr.
+
+Lemma tbl_merge_rows_2_body :
+  func_sound ge tbl_merge_rows_2_fd nil tbl_merge_rows_2_spec.
+Proof.
+  start_function.
+  table_action act_merge_rows_2_body.
+  { entailer. }
+  { entailer. }
+Qed.
+
+#[local] Hint Extern 5 (func_modifies _ _ _ _ _) => (apply tbl_merge_rows_2_body) : func_specs.
+
+Definition tbl_merge_rows_3_fd :=
+  ltac:(get_fd ["Cm2CountMinSketchWin"; "tbl_merge_rows_3"; "apply"] ge).
+
+Definition tbl_merge_rows_3_spec : func_spec :=
+  WITH (* p *),
+    PATH p
+    MOD (Some [["win_md"]]) []
+    WITH api index_1 index_2 index_3 index_4 index_5 rw_1 rw_2 rw_3 rw_4 rw_5,
+      PRE
+        (ARG []
+        (MEM [(["win_md"], ValBaseStruct
+               [("api", api);
+                ("index_1", index_1);
+                ("index_2", index_2);
+                ("index_3", index_3);
+                ("index_4", index_4);
+                ("index_5", index_5);
+                ("rw_1", P4Bit value_w rw_1);
+                ("rw_2", P4Bit value_w rw_2);
+                ("rw_3", rw_3);
+                ("rw_4", rw_4);
+                ("rw_5", rw_5)
+               ])
+             ]
+        (EXT [])))
+      POST
+        (EX retv,
+        (ARG_RET [] retv
+        (MEM [(["win_md"], ValBaseStruct
+               [("api", api);
+                ("index_1", index_1);
+                ("index_2", index_2);
+                ("index_3", index_3);
+                ("index_4", index_4);
+                ("index_5", index_5);
+                ("rw_1", P4Bit value_w (P4min rw_1 rw_2));
+                ("rw_2", P4Bit value_w rw_2);
+                ("rw_3", rw_3);
+                ("rw_4", rw_4);
+                ("rw_5", rw_5)
+               ])
+             ]
+        (EXT []))))%arg_ret_assr.
+
+Lemma tbl_merge_rows_3_body :
+  func_sound ge tbl_merge_rows_3_fd nil tbl_merge_rows_3_spec.
+Proof.
+  start_function.
+  table_action act_merge_rows_3_body.
+  { entailer. }
+  { entailer. }
+Qed.
+
+#[local] Hint Extern 5 (func_modifies _ _ _ _ _) => (apply tbl_merge_rows_3_body) : func_specs.
+
+Definition min_undef_spec : func_spec :=
+  WITH,
+    PATH []
+    MOD None []
+    WITH,
+      PRE
+        (ARG [P4Bit_ value_w; P4Bit_ value_w]
+        (MEM []
+        (EXT [])))
+      POST
+        (ARG_RET [] (P4Bit_ value_w)
+        (MEM []
+        (EXT []))).
+
+Lemma min_undef_body :
+  func_sound ge (FExternal "" "min") [TypBit value_w] min_undef_spec.
+Admitted.
+
+Definition act_merge_rows_1_undef_spec : func_spec :=
+  WITH (* p *),
+    PATH p
+    MOD (Some [["win_md"]]) []
+    WITH api index_1 index_2 index_3 index_4 index_5,
+      PRE
+        (ARG []
+        (MEM [(["win_md"], ValBaseStruct
+               [("api", api);
+                ("index_1", index_1);
+                ("index_2", index_2);
+                ("index_3", index_3);
+                ("index_4", index_4);
+                ("index_5", index_5);
+                ("rw_1", P4Bit_ value_w);
+                ("rw_2", P4Bit_ value_w);
+                ("rw_3", P4Bit_ value_w);
+                ("rw_4", P4Bit_ value_w);
+                ("rw_5", P4Bit_ value_w)
+               ])
+             ]
+        (EXT [])))
+      POST
+        (ARG_RET [] ValBaseNull
+        (MEM [(["win_md"], ValBaseStruct
+               [("api", api);
+                ("index_1", index_1);
+                ("index_2", index_2);
+                ("index_3", index_3);
+                ("index_4", index_4);
+                ("index_5", index_5);
+                ("rw_1", P4Bit_ value_w);
+                ("rw_2", P4Bit_ value_w);
+                ("rw_3", P4Bit_ value_w);
+                ("rw_4", P4Bit_ value_w);
+                ("rw_5", P4Bit_ value_w)
+               ])
+             ]
+        (EXT []))).
+
+Lemma act_merge_rows_1_undef_body :
+  func_sound ge act_merge_rows_1_fd nil act_merge_rows_1_undef_spec.
+Proof.
+  start_function.
+  step_call min_undef_body.
+  { entailer. }
+  step_call min_undef_body.
+  { entailer. }
+  step.
+  entailer.
+Qed.
+
+Definition act_merge_rows_2_undef_spec : func_spec :=
+  WITH (* p *),
+    PATH p
+    MOD (Some [["win_md"]]) []
+    WITH api index_1 index_2 index_3 index_4 index_5 rw_2 rw_4 rw_5,
+      PRE
+        (ARG []
+        (MEM [(["win_md"], ValBaseStruct
+               [("api", api);
+                ("index_1", index_1);
+                ("index_2", index_2);
+                ("index_3", index_3);
+                ("index_4", index_4);
+                ("index_5", index_5);
+                ("rw_1", P4Bit_ value_w);
+                ("rw_2", rw_2);
+                ("rw_3", P4Bit_ value_w);
+                ("rw_4", rw_4);
+                ("rw_5", rw_5)
+               ])
+             ]
+        (EXT [])))
+      POST
+        (ARG_RET [] ValBaseNull
+        (MEM [(["win_md"], ValBaseStruct
+               [("api", api);
+                ("index_1", index_1);
+                ("index_2", index_2);
+                ("index_3", index_3);
+                ("index_4", index_4);
+                ("index_5", index_5);
+                ("rw_1", P4Bit_ value_w);
+                ("rw_2", rw_2);
+                ("rw_3", P4Bit_ value_w);
+                ("rw_4", rw_4);
+                ("rw_5", rw_5)
+               ])
+             ]
+        (EXT []))).
+
+Lemma act_merge_rows_2_undef_body :
+  func_sound ge act_merge_rows_2_fd nil act_merge_rows_2_undef_spec.
+Proof.
+  start_function.
+  step_call min_undef_body.
+  { entailer. }
+  step.
+  entailer.
+Qed.
+
+Definition act_merge_rows_3_undef_spec : func_spec :=
+  WITH (* p *),
+    PATH p
+    MOD (Some [["win_md"]]) []
+    WITH api index_1 index_2 index_3 index_4 index_5 rw_3 rw_4 rw_5,
+      PRE
+        (ARG []
+        (MEM [(["win_md"], ValBaseStruct
+               [("api", api);
+                ("index_1", index_1);
+                ("index_2", index_2);
+                ("index_3", index_3);
+                ("index_4", index_4);
+                ("index_5", index_5);
+                ("rw_1", P4Bit_ value_w);
+                ("rw_2", P4Bit_ value_w);
+                ("rw_3", rw_3);
+                ("rw_4", rw_4);
+                ("rw_5", rw_5)
+               ])
+             ]
+        (EXT [])))
+      POST
+        (ARG_RET [] ValBaseNull
+        (MEM [(["win_md"], ValBaseStruct
+               [("api", api);
+                ("index_1", index_1);
+                ("index_2", index_2);
+                ("index_3", index_3);
+                ("index_4", index_4);
+                ("index_5", index_5);
+                ("rw_1", P4Bit_ value_w);
+                ("rw_2", P4Bit_ value_w);
+                ("rw_3", rw_3);
+                ("rw_4", rw_4);
+                ("rw_5", rw_5)
+               ])
+             ]
+        (EXT []))).
+
+Lemma act_merge_rows_3_undef_body :
+  func_sound ge act_merge_rows_3_fd nil act_merge_rows_3_undef_spec.
+Proof.
+  start_function.
+  step_call min_undef_body.
+  { entailer. }
+  step.
+  entailer.
+Qed.
+
+Definition tbl_merge_rows_1_undef_spec : func_spec :=
+  WITH (* p *),
+    PATH p
+    MOD (Some [["win_md"]]) []
+    WITH api index_1 index_2 index_3 index_4 index_5,
+      PRE
+        (ARG []
+        (MEM [(["win_md"], ValBaseStruct
+               [("api", api);
+                ("index_1", index_1);
+                ("index_2", index_2);
+                ("index_3", index_3);
+                ("index_4", index_4);
+                ("index_5", index_5);
+                ("rw_1", P4Bit_ value_w);
+                ("rw_2", P4Bit_ value_w);
+                ("rw_3", P4Bit_ value_w);
+                ("rw_4", P4Bit_ value_w);
+                ("rw_5", P4Bit_ value_w)
+               ])
+             ]
+        (EXT [])))
+      POST
+        (EX retv,
+        (ARG_RET [] retv
+        (MEM [(["win_md"], ValBaseStruct
+               [("api", api);
+                ("index_1", index_1);
+                ("index_2", index_2);
+                ("index_3", index_3);
+                ("index_4", index_4);
+                ("index_5", index_5);
+                ("rw_1", P4Bit_ value_w);
+                ("rw_2", P4Bit_ value_w);
+                ("rw_3", P4Bit_ value_w);
+                ("rw_4", P4Bit_ value_w);
+                ("rw_5", P4Bit_ value_w)
+               ])
+             ]
+        (EXT []))))%arg_ret_assr.
+
+Lemma tbl_merge_rows_1_undef_body :
+  func_sound ge tbl_merge_rows_1_fd nil tbl_merge_rows_1_undef_spec.
+Proof.
+  start_function.
+  table_action act_merge_rows_1_undef_body.
+  { entailer. }
+  { entailer. }
+Qed.
+
+Definition tbl_merge_rows_2_undef_spec : func_spec :=
+  WITH (* p *),
+    PATH p
+    MOD (Some [["win_md"]]) []
+    WITH api index_1 index_2 index_3 index_4 index_5 rw_2 rw_4 rw_5,
+      PRE
+        (ARG []
+        (MEM [(["win_md"], ValBaseStruct
+               [("api", api);
+                ("index_1", index_1);
+                ("index_2", index_2);
+                ("index_3", index_3);
+                ("index_4", index_4);
+                ("index_5", index_5);
+                ("rw_1", P4Bit_ value_w);
+                ("rw_2", rw_2);
+                ("rw_3", P4Bit_ value_w);
+                ("rw_4", rw_4);
+                ("rw_5", rw_5)
+               ])
+             ]
+        (EXT [])))
+      POST
+        (EX retv,
+        (ARG_RET [] retv
+        (MEM [(["win_md"], ValBaseStruct
+               [("api", api);
+                ("index_1", index_1);
+                ("index_2", index_2);
+                ("index_3", index_3);
+                ("index_4", index_4);
+                ("index_5", index_5);
+                ("rw_1", P4Bit_ value_w);
+                ("rw_2", rw_2);
+                ("rw_3", P4Bit_ value_w);
+                ("rw_4", rw_4);
+                ("rw_5", rw_5)
+               ])
+             ]
+        (EXT []))))%arg_ret_assr.
+
+Lemma tbl_merge_rows_2_undef_body :
+  func_sound ge tbl_merge_rows_2_fd nil tbl_merge_rows_2_undef_spec.
+Proof.
+  start_function.
+  table_action act_merge_rows_2_undef_body.
+  { entailer. }
+  { entailer. }
+Qed.
+
+Definition tbl_merge_rows_3_undef_spec : func_spec :=
+  WITH (* p *),
+    PATH p
+    MOD (Some [["win_md"]]) []
+    WITH api index_1 index_2 index_3 index_4 index_5 rw_3 rw_4 rw_5,
+      PRE
+        (ARG []
+        (MEM [(["win_md"], ValBaseStruct
+               [("api", api);
+                ("index_1", index_1);
+                ("index_2", index_2);
+                ("index_3", index_3);
+                ("index_4", index_4);
+                ("index_5", index_5);
+                ("rw_1", P4Bit_ value_w);
+                ("rw_2", P4Bit_ value_w);
+                ("rw_3", rw_3);
+                ("rw_4", rw_4);
+                ("rw_5", rw_5)
+               ])
+             ]
+        (EXT [])))
+      POST
+        (EX retv,
+        (ARG_RET [] retv
+        (MEM [(["win_md"], ValBaseStruct
+               [("api", api);
+                ("index_1", index_1);
+                ("index_2", index_2);
+                ("index_3", index_3);
+                ("index_4", index_4);
+                ("index_5", index_5);
+                ("rw_1", P4Bit_ value_w);
+                ("rw_2", P4Bit_ value_w);
+                ("rw_3", rw_3);
+                ("rw_4", rw_4);
+                ("rw_5", rw_5)
+               ])
+             ]
+        (EXT []))))%arg_ret_assr.
+
+Lemma tbl_merge_rows_3_undef_body :
+  func_sound ge tbl_merge_rows_3_fd nil tbl_merge_rows_3_undef_spec.
+Proof.
+  start_function.
+  table_action act_merge_rows_3_undef_body.
+  { entailer. }
+  { entailer. }
+Qed.
 
 Definition Win_fundef :=
   ltac:(get_fd ["Cm2CountMinSketchWin"; "apply"] ge).
@@ -63,7 +742,43 @@ Definition Win_noop_spec : func_spec :=
 Lemma Win_noop_body :
   func_sound ge Win_fundef nil Win_noop_spec.
 Proof.
-Admitted.
+  start_function.
+  unfold frame_repr.
+  normalize_EXT.
+  destruct f as [f ?H]. destruct is as [is ?H].
+  cbn [proj1_sig] in *.
+  destruct_list f.
+  destruct_list is.
+  repeat lazymatch goal with
+  | H : Forall _ _ |- _ => inv H
+  end.
+  step_call verif_Row21.Row_noop_case_body.
+  { entailer. }
+  { auto. }
+  step_call verif_Row22.Row_noop_case_body.
+  { entailer. }
+  { auto. }
+  step_call verif_Row23.Row_noop_case_body.
+  { entailer. }
+  { auto. }
+  step_call verif_Row24.Row_noop_case_body.
+  { entailer. }
+  { auto. }
+  step_call verif_Row25.Row_noop_case_body.
+  { entailer. }
+  { auto. }
+  step_call tbl_merge_rows_1_undef_body.
+  { entailer. }
+  Intros _.
+  step_call tbl_merge_rows_2_undef_body.
+  { entailer. }
+  Intros _.
+  step_call tbl_merge_rows_3_undef_body.
+  { entailer. }
+  Intros _.
+  step.
+  entailer.
+Qed.
 
 Definition Win_insert_spec : func_spec :=
   WITH (* p *),
@@ -109,7 +824,45 @@ Definition Win_insert_spec : func_spec :=
 Lemma Win_insert_body :
   func_sound ge Win_fundef nil Win_insert_spec.
 Proof.
-Admitted.
+  start_function.
+  unfold frame_repr.
+  normalize_EXT.
+  destruct f as [f ?H]. destruct is as [is ?H].
+  cbn [proj1_sig frame_insert] in *.
+  destruct_list f.
+  destruct_list is.
+  repeat lazymatch goal with
+  | H : Forall _ _ |- _ => inv H
+  end.
+  step_call verif_Row21.Row_insert_case_body.
+  { entailer. }
+  { auto. }
+  step_call verif_Row22.Row_insert_case_body.
+  { entailer. }
+  { auto. }
+  step_call verif_Row23.Row_insert_case_body.
+  { entailer. }
+  { auto. }
+  step_call verif_Row24.Row_insert_case_body.
+  { entailer. }
+  { auto. }
+  step_call verif_Row25.Row_insert_case_body.
+  { entailer. }
+  { auto. }
+  step_call tbl_merge_rows_1_undef_body.
+  { entailer.
+    repeat constructor.
+  }
+  Intros _.
+  step_call tbl_merge_rows_2_undef_body.
+  { entailer. }
+  Intros _.
+  step_call tbl_merge_rows_3_undef_body.
+  { entailer. }
+  Intros _.
+  step.
+  entailer.
+Qed.
 
 Definition Win_query_spec : func_spec :=
   WITH (* p *),
@@ -152,10 +905,92 @@ Definition Win_query_spec : func_spec :=
         (MEM []
         (EXT [frame_repr p rows f]))).
 
+(* A very slow test case in "apply" unless makeing row_repr opaque. *)
+(* Lemma test : forall (x x0 : row), exists p0,
+  ext_implies [row_repr (p ++ ["row_1"]) x] [row_repr p0 x0].
+Proof.
+  intros. eexists.
+  apply ext_implies_refl. *)
+
 Lemma Win_query_body :
   func_sound ge Win_fundef nil Win_query_spec.
 Proof.
-Admitted.
+  start_function.
+  unfold frame_repr.
+  normalize_EXT.
+  destruct f as [f ?H]. destruct is as [is ?H].
+  cbn [proj1_sig] in *.
+  destruct_list f.
+  destruct_list is.
+  repeat lazymatch goal with
+  | H : Forall _ _ |- _ => inv H
+  end.
+
+Ltac pose_row_query_bound r i :=
+  P4assert (row_query r i >= 0);
+  only 1 : (
+    eapply ext_implies_trans;
+    only 2 : (apply row_query_bound; auto);
+    entailer
+  ).
+
+  Opaque row_repr.
+  pose_row_query_bound x x4.
+  pose_row_query_bound x0 x5.
+  pose_row_query_bound x1 x6.
+  pose_row_query_bound x2 x7.
+  pose_row_query_bound x3 x8.
+  Transparent row_repr.
+
+  step_call verif_Row21.Row_query_case_body.
+  { entailer. }
+  { auto. }
+  step_call verif_Row22.Row_query_case_body.
+  { entailer. }
+  { auto. }
+  step_call verif_Row23.Row_query_case_body.
+  { entailer. }
+  { auto. }
+  step_call verif_Row24.Row_query_case_body.
+  { entailer. }
+  { auto. }
+  step_call verif_Row25.Row_query_case_body.
+  { entailer. }
+  { auto. }
+  step_call tbl_merge_rows_1_body.
+  { entailer. }
+  Intros _.
+  step_call tbl_merge_rows_2_body.
+  { entailer. }
+  Intros _.
+  step_call tbl_merge_rows_3_body.
+  { entailer. }
+  Intros _.
+  step.
+  entailer.
+  constructor.
+  repeat first [
+    apply Forall2_nil
+  | apply Forall2_cons; only 1 : (split; only 1 : reflexivity);
+    try apply sval_refine_refl
+  ].
+  2-5 : repeat constructor.
+  apply sval_refine_refl'. do 3 f_equal.
+  unfold P4min.
+  change (Znth 0 [x4; x5; x6; x7; x8]) with x4.
+  change (Znth 1 [x4; x5; x6; x7; x8]) with x5.
+  change (Znth 2 [x4; x5; x6; x7; x8]) with x6.
+  change (Znth 3 [x4; x5; x6; x7; x8]) with x7.
+  change (Znth 4 [x4; x5; x6; x7; x8]) with x8.
+  unfold value_w.
+  rewrite_strat bottomup mod_bound_small.
+  2-9 : lia.
+  unfold frame_query.
+  simpl Utils.list_min.
+  repeat rewrite Zmin_shrink.
+  f_equal.
+  lia.
+Qed.
 
 Definition Win_clear_spec : func_spec :=
   WITH (* p *),
@@ -201,7 +1036,50 @@ Definition Win_clear_spec : func_spec :=
 Lemma Win_clear_body :
   func_sound ge Win_fundef nil Win_clear_spec.
 Proof.
-Admitted.
+  start_function.
+  unfold frame_repr.
+  normalize_EXT.
+  destruct f as [f ?H]. destruct is as [is ?H].
+  cbn [proj1_sig frame_clear] in *.
+  destruct_list f.
+  destruct_list is.
+  repeat lazymatch goal with
+  | H : Forall _ _ |- _ => inv H
+  end.
+  step_call verif_Row21.Row_clear_case_body.
+  { entailer. }
+  { auto. }
+  step_call verif_Row22.Row_clear_case_body.
+  { entailer. }
+  { auto. }
+  step_call verif_Row23.Row_clear_case_body.
+  { entailer. }
+  { auto. }
+  step_call verif_Row24.Row_clear_case_body.
+  { entailer. }
+  { auto. }
+  step_call verif_Row25.Row_clear_case_body.
+  { entailer. }
+  { auto. }
+  step_call tbl_merge_rows_1_body.
+  { entailer. }
+  Intros _.
+  step_call tbl_merge_rows_2_body.
+  { entailer. }
+  Intros _.
+  step_call tbl_merge_rows_3_body.
+  { entailer. }
+  Intros _.
+  step.
+  entailer.
+  constructor.
+  repeat first [
+    apply Forall2_nil
+  | apply Forall2_cons; only 1 : (split; only 1 : reflexivity);
+    try apply sval_refine_refl
+  ];
+  repeat constructor.
+Qed.
 
 #[export] Hint Extern 5 (func_modifies _ _ _ _ _) => (apply Win_noop_body) : func_specs.
 
