examples/sbf/verif_Row23.v
@@ -1,0 +1,415 @@
+Require Import Poulet4.P4light.Syntax.P4defs.
+Require Import Poulet4.P4light.Semantics.Semantics.
+Require Import ProD3.core.Core.
+Require Import ProD3.core.Tofino.
+Require Import ProD3.examples.sbf.p4ast.
+Require Import ProD3.examples.sbf.ConFilter.
+Require Import ProD3.examples.sbf.common.
+Require Import ProD3.examples.sbf.FilterRepr.
+Require Import Hammer.Plugin.Hammer.
+Import ListNotations.
+
+Notation ident := string.
+Notation path := (list ident).
+Notation Val := (@ValueBase bool).
+Notation Sval := (@ValueBase (option bool)).
+
+Definition p := ["pipe"; "ingress"; "bf2_ds"; "win_2"; "row_3"].
+
+Open Scope func_spec.
+
+Definition Row_regact_insert_apply_body :=
+  ltac:(auto_regact ge am_ge (p ++ ["regact_insert"])).
+
+(* I would like to make it opaque, but I don't know how to. *)
+Definition Row_regact_insert_execute_body :=
+  ltac:(build_execute_body ge Row_regact_insert_apply_body).
+
+#[local] Hint Extern 5 (func_modifies _ _ _ _ _) => (apply Row_regact_insert_execute_body) : func_specs.
+
+Definition Row_insert_fundef :=
+  ltac:(get_fd ["Bf2BloomFilterRow"; "act_insert"] ge).
+
+(* Program:
+  action act_insert() {
+      rw = regact_insert.execute(index);
+  }
+*)
+
+Definition Row_insert_spec : func_spec :=
+  WITH (* p *),
+    PATH p
+    MOD (Some [["rw"]]) [p]
+    WITH (r : row) (i : Z)
+      (_ : 0 <= i < num_slots),
+      PRE
+        (ARG []
+        (MEM [(["index"], P4Bit index_w i)]
+        (EXT [row_repr p r])))
+      POST
+        (ARG_RET [] ValBaseNull
+        (MEM [(["rw"], P4Bit 8 1)]
+        (EXT [row_repr p (row_insert r i)]))).
+
+Lemma Row_insert_body :
+  func_sound ge Row_insert_fundef nil Row_insert_spec.
+Proof.
+  start_function.
+  destruct r as [r ?H].
+  unfold row_repr, row_reg_repr. cbn [proj1_sig row_insert].
+  normalize_EXT.
+  step_call Row_regact_insert_execute_body.
+  { entailer. }
+  { list_solve. }
+  { lia. }
+  { rewrite Znth_map by list_solve.
+    reflexivity.
+  }
+  step.
+  entailer.
+  f_equal.
+  list_solve.
+Qed.
+
+#[local] Hint Extern 5 (func_modifies _ _ _ _ _) => (apply Row_insert_body) : func_specs.
+
+Definition Row_regact_query_apply_body :=
+  ltac:(auto_regact ge am_ge (p ++ ["regact_query"])).
+
+Definition Row_regact_query_execute_body :=
+  ltac:(build_execute_body ge Row_regact_query_apply_body).
+
+#[local] Hint Extern 5 (func_modifies _ _ _ _ _) => (apply Row_regact_query_execute_body) : func_specs.
+
+Definition Row_query_fundef := Eval compute in
+  ltac:(get_fd ["Bf2BloomFilterRow"; "act_query"] ge).
+
+(* Program:
+  action act_query() {
+      rw = regact_query.execute(index);
+  }
+*)
+
+Definition Row_query_spec : func_spec :=
+  WITH (* p *),
+    PATH p
+    MOD (Some [["rw"]]) [p]
+    WITH (r : row) (i : Z)
+      (_ : 0 <= i < num_slots),
+      PRE
+        (ARG []
+        (MEM [(["index"], P4Bit index_w i)]
+        (EXT [row_repr p r])))
+      POST
+        (ARG_RET [] ValBaseNull
+        (MEM [(["rw"], P4Bit 8 (Z.b2z (row_query r i)))]
+        (EXT [row_repr p r]))).
+
+Lemma Row_query_body :
+  func_sound ge Row_query_fundef nil Row_query_spec.
+Proof.
+  start_function.
+  destruct r as [r ?H].
+  unfold row_repr, row_reg_repr. cbn [proj1_sig].
+  normalize_EXT.
+  step_call Row_regact_query_execute_body.
+  { entailer. }
+  { list_solve. }
+  { lia. }
+  { rewrite Znth_map by list_solve.
+    reflexivity.
+  }
+  step.
+  entailer.
+  { f_equal.
+    list_simplify. subst. auto.
+  }
+Qed.
+
+#[local] Hint Extern 5 (func_modifies _ _ _ _ _) => (apply Row_query_body) : func_specs.
+
+Definition Row_regact_clear_apply_body :=
+  ltac:(auto_regact ge am_ge (p ++ ["regact_clear"])).
+
+(* Finished transaction in 0.179 secs (0.14u,0.031s) (successful) *)
+Definition Row_regact_clear_execute_body :=
+  ltac:(build_execute_body ge Row_regact_clear_apply_body).
+
+#[local] Hint Extern 5 (func_modifies _ _ _ _ _) => (apply Row_regact_clear_execute_body) : func_specs.
+
+Definition Row_clear_fundef :=
+  ltac:(get_fd ["Bf2BloomFilterRow"; "act_clear"] ge).
+
+(* Program:
+  action act_clear() {
+      rw = regact_clear.execute(index);
+  }
+*)
+
+Definition Row_clear_spec : func_spec :=
+  WITH (* p *),
+    PATH p
+    MOD (Some [["rw"]]) [p]
+    WITH (r : row) (i : Z)
+      (_ : 0 <= i < num_slots),
+      PRE
+        (ARG []
+        (MEM [(["index"], P4Bit index_w i)]
+        (EXT [row_repr p r])))
+      POST
+        (ARG_RET [] ValBaseNull
+        (MEM [(["rw"], P4Bit 8 0)]
+        (EXT [row_repr p (row_clear r i)]))).
+
+Lemma Row_clear_body :
+  func_sound ge Row_clear_fundef nil Row_clear_spec.
+Proof.
+  start_function.
+  destruct r as [r ?H].
+  unfold row_repr, row_reg_repr. cbn [proj1_sig row_clear].
+  normalize_EXT.
+  step_call Row_regact_clear_execute_body.
+  { entailer. }
+  { list_solve. }
+  { lia. }
+  { rewrite Znth_map by list_solve.
+    reflexivity.
+  }
+  step.
+  entailer.
+  f_equal.
+  list_solve.
+Qed.
+
+#[local] Hint Extern 5 (func_modifies _ _ _ _ _) => (apply Row_clear_body) : func_specs.
+
+Definition Row_tbl_bloom_fundef :=
+  ltac:(get_fd ["Bf2BloomFilterRow"; "tbl_bloom"; "apply"] ge).
+
+Definition Row_fundef :=
+  ltac:(get_fd ["Bf2BloomFilterRow"; "apply"] ge).
+
+Definition Row_noop_case_spec : func_spec :=
+  WITH (* p *),
+    PATH p
+    MOD None [p]
+    WITH (r : row) (i : Z)
+      (_ : 0 <= i < num_slots),
+      PRE
+        (ARG [P4Bit 8 NOOP;
+              P4Bit index_w i]
+        (MEM []
+        (EXT [row_repr p r])))
+      POST
+        (ARG_RET [P4Bit_ 8] ValBaseNull
+        (MEM []
+        (EXT [row_repr p r]))).
+
+Definition Row_tbl_bloom_noop_spec : func_spec :=
+  WITH (* p *),
+    PATH p
+    MOD (Some [["rw"]]) [p]
+    WITH (r : row),
+      PRE
+        (ARG []
+        (MEM [(["api"], P4Bit 8 NOOP);
+              (["rw"], P4Bit_ 8)]
+        (EXT [row_repr p r])))
+      POST
+        (EX retv,
+        (ARG_RET [] retv
+        (MEM [(["rw"], P4Bit_ 8)]
+        (EXT [row_repr p r]))))%arg_ret_assr.
+
+Lemma Row_tbl_bloom_noop_body :
+  func_sound ge Row_tbl_bloom_fundef nil Row_tbl_bloom_noop_spec.
+Proof.
+  start_function; elim_trivial_cases; try lia.
+  table_action NoAction_body.
+  { entailer. }
+  { entailer. }
+Qed.
+
+Lemma Row_noop_case_body :
+  func_sound ge Row_fundef nil Row_noop_case_spec.
+Proof.
+  start_function.
+  step.
+  step_call Row_tbl_bloom_noop_body.
+  { entailer. }
+  Intros _.
+  step.
+  entailer.
+Qed.
+
+#[export] Hint Extern 5 (func_modifies _ _ _ _ _) => (apply Row_noop_case_body) : func_specs.
+
+Definition Row_insert_case_spec : func_spec :=
+  WITH (* p *),
+    PATH p
+    MOD None [p]
+    WITH (r : row) (i : Z)
+      (_ : 0 <= i < num_slots),
+      PRE
+        (ARG [P4Bit 8 INSERT;
+              P4Bit index_w i]
+        (MEM []
+        (EXT [row_repr p r])))
+      POST
+        (ARG_RET [P4Bit 8 1] ValBaseNull
+        (MEM []
+        (EXT [row_repr p (row_insert r i)]))).
+
+Definition Row_tbl_bloom_insert_spec : func_spec :=
+  WITH (* p *),
+    PATH p
+    MOD (Some [["rw"]]) [p]
+    WITH (r : row) (i : Z)
+      (_ : 0 <= i < num_slots),
+      PRE
+        (ARG []
+        (MEM [(["api"], P4Bit 8 INSERT);
+              (["index"], P4Bit index_w i)]
+        (EXT [row_repr p r])))
+      POST
+        (EX retv,
+        (ARG_RET [] retv
+        (MEM [(["rw"], P4Bit 8 1)]
+        (EXT [row_repr p (row_insert r i)]))))%arg_ret_assr.
+
+Lemma Row_tbl_bloom_insert_body :
+  func_sound ge Row_tbl_bloom_fundef nil Row_tbl_bloom_insert_spec.
+Proof.
+  start_function; elim_trivial_cases; try lia.
+  table_action Row_insert_body.
+  { entailer. }
+  { auto. }
+  { entailer. }
+Qed.
+
+Lemma Row_insert_case_body :
+  func_sound ge Row_fundef nil Row_insert_case_spec.
+Proof.
+  start_function.
+  step.
+  step_call Row_tbl_bloom_insert_body.
+  { entailer. }
+  { auto. }
+  Intros _.
+  step.
+  entailer.
+Qed.
+
+Definition Row_query_case_spec : func_spec :=
+  WITH (* p *),
+    PATH p
+    MOD None [p]
+    WITH (r : row) (i : Z)
+      (_ : 0 <= i < num_slots),
+      PRE
+        (ARG [P4Bit 8 QUERY;
+              P4Bit index_w i]
+        (MEM []
+        (EXT [row_repr p r])))
+      POST
+        (ARG_RET [P4Bit 8 (Z.b2z (row_query r i))] ValBaseNull
+        (MEM []
+        (EXT [row_repr p r]))).
+
+Definition Row_tbl_bloom_query_spec : func_spec :=
+  WITH (* p *),
+    PATH p
+    MOD (Some [["rw"]]) [p]
+    WITH (r : row) (i : Z)
+      (_ : 0 <= i < num_slots),
+      PRE
+        (ARG []
+        (MEM [(["api"], P4Bit 8 QUERY);
+              (["index"], P4Bit index_w i)]
+        (EXT [row_repr p r])))
+      POST
+        (EX retv,
+        (ARG_RET [] retv
+        (MEM [(["rw"], P4Bit 8 (Z.b2z (row_query r i)))]
+        (EXT [row_repr p r]))))%arg_ret_assr.
+
+Lemma Row_tbl_bloom_query_body :
+  func_sound ge Row_tbl_bloom_fundef nil Row_tbl_bloom_query_spec.
+Proof.
+  start_function; elim_trivial_cases; try lia.
+  table_action Row_query_body.
+  { entailer. }
+  { auto. }
+  { entailer. }
+Qed.
+
+Lemma Row_query_case_body :
+  func_sound ge Row_fundef nil Row_query_case_spec.
+Proof.
+  start_function.
+  step.
+  step_call Row_tbl_bloom_query_body.
+  { entailer. }
+  { auto. }
+  Intros _.
+  step.
+  entailer.
+Qed.
+
+Definition Row_clear_case_spec : func_spec :=
+  WITH (* p *),
+    PATH p
+    MOD None [p]
+    WITH (r : row) (i : Z)
+      (_ : 0 <= i < num_slots),
+      PRE
+        (ARG [P4Bit 8 CLEAR;
+              P4Bit index_w i]
+        (MEM []
+        (EXT [row_repr p r])))
+      POST
+        (ARG_RET [P4Bit 8 0] ValBaseNull
+        (MEM []
+        (EXT [row_repr p (row_clear r i)]))).
+
+Definition Row_tbl_bloom_clear_spec : func_spec :=
+  WITH (* p *),
+    PATH p
+    MOD (Some [["rw"]]) [p]
+    WITH (r : row) (i : Z)
+      (_ : 0 <= i < num_slots),
+      PRE
+        (ARG []
+        (MEM [(["api"], P4Bit 8 CLEAR);
+              (["index"], P4Bit index_w i)]
+        (EXT [row_repr p r])))
+      POST
+        (EX retv,
+        (ARG_RET [] retv
+        (MEM [(["rw"], P4Bit 8 0)]
+        (EXT [row_repr p (row_clear r i)]))))%arg_ret_assr.
+
+Lemma Row_tbl_bloom_clear_body :
+  func_sound ge Row_tbl_bloom_fundef nil Row_tbl_bloom_clear_spec.
+Proof.
+  start_function; elim_trivial_cases; try lia.
+  table_action Row_clear_body.
+  { entailer. }
+  { auto. }
+  { entailer. }
+Qed.
+
+Lemma Row_clear_case_body :
+  func_sound ge Row_fundef nil Row_clear_case_spec.
+Proof.
+  start_function.
+  step.
+  step_call Row_tbl_bloom_clear_body.
+  { entailer. }
+  { auto. }
+  Intros _.
+  step.
+  entailer.
+Qed.
+
+#[export] Hint Extern 5 (func_modifies _ _ _ _ _) => (apply Row_noop_case_body) : func_specs.
